backend/LTL.v
@@ -242,24 +242,23 @@ Inductive step: state -> trace -> state -> Prop :=
       find_function ros rs = Some fd ->
       funsig fd = sig ->
       step (Block s f sp (Lcall sig ros :: bb) rs m)
-        E0 (Callstate (Stackframe f sp rs bb :: s) fd rs
-                      (Mem.push_stage m)
+        E0 (Callstate (Stackframe f sp rs bb :: s) fd rs m
                       (fn_stack_requirements id))
-  | exec_Ltailcall: forall s f sp sig ros bb rs m fd rs' m' id,
+  | exec_Ltailcall: forall s f sp sig ros bb rs m fd rs' m' m'' id,
       ros_is_function ros rs id ->
       rs' = return_regs (parent_locset s) rs ->
       find_function ros rs' = Some fd ->
       funsig fd = sig ->
       Mem.free m sp 0 f.(fn_stacksize) = Some m' ->
-      step (Block s f (Vptr sp Ptrofs.zero) (Ltailcall sig ros :: bb) rs m)
-        E0 (Callstate s fd rs' m' (fn_stack_requirements id))
-  | exec_Lbuiltin: forall s f sp ef args res bb rs m vargs t vres rs' m' m'',
-      eval_builtin_args ge rs sp m args vargs ->
-      external_call ef ge vargs (Mem.push_stage m) t vres m' ->
       Mem.pop_stage m' = Some m'' ->
+      step (Block s f (Vptr sp Ptrofs.zero) (Ltailcall sig ros :: bb) rs m)
+        E0 (Callstate s fd rs' m'' (fn_stack_requirements id))
+  | exec_Lbuiltin: forall s f sp ef args res bb rs m vargs t vres rs' m',
+      eval_builtin_args ge rs sp m args vargs ->
+      external_call ef ge vargs m t vres m' ->
       rs' = Locmap.setres res vres (undef_regs (destroyed_by_builtin ef) rs) ->
       step (Block s f sp (Lbuiltin ef args res :: bb) rs m)
-         t (Block s f sp bb rs' m'')
+         t (Block s f sp bb rs' m')
   | exec_Lbranch: forall s f sp pc bb rs m,
       step (Block s f sp (Lbranch pc :: bb) rs m)
         E0 (State s f sp pc rs m)
@@ -275,13 +274,14 @@ Inductive step: state -> trace -> state -> Prop :=
       rs' = undef_regs (destroyed_by_jumptable) rs ->
       step (Block s f sp (Ljumptable arg tbl :: bb) rs m)
         E0 (State s f sp pc rs' m)
-  | exec_Lreturn: forall s f sp bb rs m m',
+  | exec_Lreturn: forall s f sp bb rs m m' m'',
       Mem.free m sp 0 f.(fn_stacksize) = Some m' ->
+      Mem.pop_stage m' = Some m'' ->
       step (Block s f (Vptr sp Ptrofs.zero) (Lreturn :: bb) rs m)
-        E0 (Returnstate s (return_regs (parent_locset s) rs) m')
+        E0 (Returnstate s (return_regs (parent_locset s) rs) m'')
   | exec_function_internal: forall s f rs m m' m'' sp rs' sz,
       Mem.alloc m 0 f.(fn_stacksize) = (m', sp) ->
-      Mem.record_frame_mach m' (Mem.mk_frame sz) = Some m'' ->
+      Mem.record_frame_mach (Mem.push_stage m') (Mem.mk_frame sz) = Some m'' ->
       rs' = undef_regs destroyed_at_function_entry (call_regs rs) ->
       step (Callstate s (Internal f) rs m sz)
         E0 (State s f (Vptr sp Ptrofs.zero) f.(fn_entrypoint) rs' m'')
@@ -291,10 +291,9 @@ Inductive step: state -> trace -> state -> Prop :=
       rs' = Locmap.setpair (loc_result (ef_sig ef)) res (undef_caller_save_regs rs) ->
       step (Callstate s (External ef) rs m sz)
          t (Returnstate s rs' m')
-  | exec_return: forall f sp rs1 bb s rs m m',
-      Mem.pop_stage m = Some m' ->
+  | exec_return: forall f sp rs1 bb s rs m,
       step (Returnstate (Stackframe f sp rs1 bb :: s) rs m)
-        E0 (Block s f sp bb rs m').
+        E0 (Block s f sp bb rs m).
 
 End RELSEM.
 
@@ -310,7 +309,7 @@ Inductive initial_state (p: program): state -> Prop :=
       Genv.find_symbol ge p.(prog_main) = Some b ->
       Genv.find_funct_ptr ge b = Some f ->
       funsig f = signature_main ->
-      initial_state p (Callstate nil f (Locmap.init Vundef) (Mem.push_stage m0)
+      initial_state p (Callstate nil f (Locmap.init Vundef) m0
                        (fn_stack_requirements (prog_main p))).
 
 Inductive final_state: state -> int -> Prop :=
