backend/Liveness.v
@@ -1,3 +1,4 @@
+
 (* *********************************************************************)
 (*                                                                     *)
 (*              The Compcert verified compiler                         *)
@@ -18,7 +19,7 @@ Require Import Lattice.
 Require Import AST.
 Require Import Op.
 Require Import Registers.
-Require Import RTL RTLmach.
+Require Import RTL RTLmach1.
 Require Import Kildall.
 
 (** A register [r] is live at a point [p] if there exists a path
